Makefile
@@ -38,7 +38,7 @@ general/dd_fc.vo \
 general/List_lemmasT.vo \
 general/swappedT.vo 
 
-ljt/ljt.vo: ljt/ljt.v general/swappedT.vo general/List_lemmasT.vo general/gstep.vo general/gen_seq.vo
+ljt/ljt.vo: ljt/ljt.v general/swappedT.vo general/gstep.vo general/gen_seq.vo 
 ljt/ljt_inv.vo: ljt/ljt_inv.v ljt/ljt.vo
 ljt/ljt_ctr.vo: ljt/ljt_ctr.v ljt/ljt_inv.vo 
 ljt/ljt_ca.vo: ljt/ljt_ca.v ljt/ljt_ctr.vo
@@ -46,7 +46,7 @@ ljt/ljt_dn.vo: ljt/ljt_dn.v ljt/ljt_inv.vo
 ljt/ljt_dncc.vo: ljt/ljt_dncc.v ljt/ljt_dn.vo ljt/ljt_ca.vo
 ljt/ljt_dnca.vo: ljt/ljt_dnca.v ljt/ljt_dncc.vo ljt/ljt_ca.vo
 ljt/ljt_dnterm.vo: ljt/ljt_dnterm.v ljt/ljt.vo general/rtcT.vo 
-ll/ll_camq.vo: ll/ll_camq.v general/dd_fc.vo general/swappedT.vo ll/fmlsext.vo ll/lldefs.vo ll/ll_lems.vo ll/ll_exch.vo ll/ll_cam.vo
+ll/ll_camq.vo: ll/ll_camq.v general/dd_fc.vo ll/fmlsext.vo ll/lldefs.vo ll/ll_lems.vo ll/ll_exch.vo ll/ll_cam.vo
 ll/ll_cam.vo: ll/ll_cam.v general/swappedT.vo general/gentree.vo
 ll/ll_ca.vo: ll/ll_ca.v general/ddT.vo
 ll/lldefs.vo: ll/lldefs.v ll/fmlsext.vo general/gstep.vo
@@ -56,8 +56,8 @@ ll/ll.vo: ll/ll.v general/ddT.vo general/swappedT.vo
 ll/fmlsext.vo: ll/fmlsext.v general/ddT.vo general/gen_tacs.vo general/List_lemmasT.vo 
 modal/k4_ca.vo: modal/k4_ca.v general/gen_tacs.vo general/gen_seq.vo general/gentree.vo modal/k4_ctr.vo
 modal/k4_ctr.vo: modal/k4_ctr.v general/gstep.vo modal/k4_inv.vo
-modal/k4_inv.vo: modal/k4_inv.v general/gstep.vo modal/k4_exch.vo
-modal/k4_exch.vo: modal/k4_exch.v general/gstep.vo general/swappedT.vo modal/k4.vo
+modal/k4_inv.vo: modal/k4_inv.v modal/k4_exch.vo
+modal/k4_exch.vo: modal/k4_exch.v general/swappedT.vo modal/k4.vo
 modal/k4.vo: modal/k4.v general/gstep.vo modal/gen_ext.vo general/List_lemmasT.vo 
 modal/gen_ext.vo: modal/gen_ext.v general/genT.vo general/gen_seq.vo
 general/gentree.vo: general/gentree.v general/gstep.vo
